coq/InSegment.v
@@ -12,96 +12,76 @@ Require Import Newton.
 
 Theorem points_in_any_newton_segment₁ : ∀ ns pts,
   Sorted fst_lt pts
-  → ns ∈ lower_convex_hull_points pts
+  → lower_convex_hull_points pts = Some ns
     → ∀ h αh, (h, αh) ∈ [ini_pt ns; fin_pt ns … oth_pts ns]
       → β ns == αh + h * γ ns.
 Proof.
 intros ns pts Hsort Hns h αh Hαh.
 unfold lower_convex_hull_points in Hns.
-remember (length pts) as n; clear Heqn.
-remember (next_ch_points n pts) as nsl eqn:Hnsl .
-revert ns pts n h αh Hsort Hnsl Hns Hαh.
-induction nsl as [| ns₁]; intros; [ contradiction | idtac ].
-destruct Hns as [Hns| Hns].
- subst ns.
- destruct n; [ discriminate Hnsl | simpl in Hnsl ].
- destruct pts as [| pt₁]; [ discriminate Hnsl | idtac ].
- destruct pts as [| pt₂]; [ discriminate Hnsl | idtac ].
- injection Hnsl; clear Hnsl; intros Hnsl Hns₁; subst nsl.
- rewrite Hns₁ in Hαh.
- remember cons as f; simpl in Hαh; subst f.
- remember (minimise_slope pt₁ pt₂ pts) as ms eqn:Hms .
+destruct pts as [| pt₁]; [ easy | idtac ].
+destruct pts as [| pt₂]; [ easy | idtac ].
+injection Hns; clear Hns; intros Hns.
+remember (minimise_slope pt₁ pt₂ pts) as ms eqn:Hms .
+destruct Hαh as [Hαh| Hαh].
+ now subst ns; unfold β, γ; rewrite Hαh.
+
  destruct Hαh as [Hαh| Hαh].
-  subst ns₁; rewrite Hαh; simpl.
-  reflexivity.
+  subst ns; simpl in Hαh; simpl.
+  rewrite Hαh; simpl.
+  unfold β, γ; simpl.
+  field.
+  apply Qgt_0_not_0, Qlt_minus.
+  remember (beg_pt ms) as pt₄.
+  remember Heqpt₄ as H; clear HeqH.
+  rewrite Hms in Heqpt₄.
+  rewrite minimised_slope_beg_pt in Heqpt₄.
+  subst pt₄ pt₁.
+  remember (fst (end_pt ms)) as x.
+  remember Heqx as H; clear HeqH.
+  rewrite Hαh in Heqx; simpl in Heqx.
+  subst x h.
+  eapply beg_lt_end_pt; [ eassumption | symmetry; eassumption ].
 
-  destruct Hαh as [Hαh| Hαh].
-   subst ns₁; simpl.
-   rewrite Hαh; simpl.
-   unfold β, γ; simpl.
-   field.
-   apply Qgt_0_not_0, Qlt_minus.
-   remember (beg_pt ms) as pt₄.
-   remember Heqpt₄ as H; clear HeqH.
-   rewrite Hms in Heqpt₄.
-   rewrite minimised_slope_beg_pt in Heqpt₄.
-   subst pt₄ pt₁.
-   remember (fst (end_pt ms)) as x.
-   remember Heqx as H; clear HeqH.
-   rewrite Hαh in Heqx; simpl in Heqx.
-   subst x h.
-   eapply beg_lt_end_pt; [ eassumption | symmetry; eassumption ].
+  subst ns; simpl in Hαh.
+  unfold β, γ; simpl.
+  revert pt₁ pt₂ h αh ms Hms Hsort Hαh.
+  induction pts as [| pt₃]; intros.
+   simpl in Hms.
+   subst ms; contradiction.
 
-   clear IHnsl.
-   subst ns₁.
-   unfold β, γ; simpl.
-   revert pt₁ pt₂ n h αh ms Hms Hsort Hαh.
-   induction pts as [| pt₃]; intros.
-    simpl in Hms.
+   simpl in Hms.
+   remember (minimise_slope pt₁ pt₃ pts) as ms₁ eqn:Hms₁ .
+   remember (slope_expr pt₁ pt₂ ?= slope ms₁) as c.
+   symmetry in Heqc.
+   rewrite slope_slope_expr in Heqc; [ idtac | symmetry; eassumption ].
+   destruct c.
+    subst ms.
+    simpl in Hαh; simpl.
+    apply Qeq_alt in Heqc.
+    unfold slope_expr in Heqc.
+    destruct Hαh as [Hαh| Hαh].
+     subst pt₂.
+     simpl in Heqc; simpl.
+     do 2 rewrite Qdiv_minus_distr_r in Heqc.
+     rewrite Qdiv_minus_distr_r.
+     apply Qeq_opp_r in Heqc.
+     do 2 rewrite Qopp_minus in Heqc.
+     rewrite <- Heqc.
+     field.
+     apply Sorted_inv_2 in Hsort; destruct Hsort as (Hlt, Hsort).
+     apply Qgt_0_not_0, Qlt_minus; assumption.
+
+     replace pt₁ with (beg_pt ms₁) .
+      eapply IHpts; try eassumption.
+      eapply Sorted_minus_2nd; [ idtac | eassumption ].
+      intros x y z H₁ H₂; eapply Qlt_trans; eassumption.
+
+      rewrite Hms₁, minimised_slope_beg_pt; reflexivity.
+
     subst ms; contradiction.
 
-    simpl in Hms.
-    remember (minimise_slope pt₁ pt₃ pts) as ms₁ eqn:Hms₁ .
-    remember (slope_expr pt₁ pt₂ ?= slope ms₁) as c.
-    symmetry in Heqc.
-    rewrite slope_slope_expr in Heqc; [ idtac | symmetry; eassumption ].
-    destruct c.
-     subst ms.
-     simpl in Hαh; simpl.
-     apply Qeq_alt in Heqc.
-     unfold slope_expr in Heqc.
-     destruct Hαh as [Hαh| Hαh].
-      subst pt₂.
-      simpl in Heqc; simpl.
-      do 2 rewrite Qdiv_minus_distr_r in Heqc.
-      rewrite Qdiv_minus_distr_r.
-      apply Qeq_opp_r in Heqc.
-      do 2 rewrite Qopp_minus in Heqc.
-      rewrite <- Heqc.
-      field.
-      apply Sorted_inv_2 in Hsort; destruct Hsort as (Hlt, Hsort).
-      apply Qgt_0_not_0, Qlt_minus; assumption.
-
-      replace pt₁ with (beg_pt ms₁) .
-       eapply IHpts; try eassumption.
-       eapply Sorted_minus_2nd; [ idtac | eassumption ].
-       intros x y z H₁ H₂; eapply Qlt_trans; eassumption.
-
-       rewrite Hms₁, minimised_slope_beg_pt; reflexivity.
-
-     subst ms; contradiction.
-
-     subst ms.
-     eapply IHpts; try eassumption.
-     eapply Sorted_minus_2nd; [ idtac | eassumption ].
-     intros x y z H₁ H₂; eapply Qlt_trans; eassumption.
-
- destruct n; [ discriminate Hnsl | simpl in Hnsl ].
- destruct pts as [| pt₁]; [ discriminate Hnsl | idtac ].
- destruct pts as [| pt₂]; [ discriminate Hnsl | idtac ].
- injection Hnsl; clear Hnsl; intros; subst ns₁ nsl.
- remember (minimise_slope pt₁ pt₂ pts) as ms eqn:Hms .
- eapply IHnsl; try reflexivity; try assumption.
- eapply minimise_slope_sorted; [ eassumption | idtac ].
- symmetry; assumption.
+    subst ms.
+    eapply IHpts; try eassumption.
+    eapply Sorted_minus_2nd; [ idtac | eassumption ].
+    intros x y z H₁ H₂; eapply Qlt_trans; eassumption.
 Qed.
